

XRAY Loss 4 Nov 2020

$$L_{\text{cEL}}(f(x), y) = \beta_p \sum_{y=1} -\ln(f(x, y)) + \beta_n \sum_{y=0} -\ln(1 - f(x, y))$$

$$\beta_p = \frac{|P| + |N|}{|P|} \quad \beta_n = \frac{|P| + |N|}{|N|} \quad \text{Jeweils um Betrag}$$

Temperatur $x = f(x)$ $z = \text{label}$

- ① $z * -\log(\sigma(x)) + (1-z) * -\log(1 - \sigma(x))$
- ② $z * -\log(1 / (1 + e^{-x})) + (1-z) * -\log(e^{-x} / (1 + e^{-x}))$
- ③ $z * \log(1 + e^{-x}) + (1-z) * (-\log(e^{-x}) + \log(1 + e^{-x}))$
- ④ $z * \log(1 + e^{-x}) + (1-z) * (x + \log(1 + e^{-x}))$
- ⑤ $(1-z) * x + \log(1 + e^{-x})$
- ⑥ $x - xz + \log(1 + e^{-x})$

$x > 0$ ⑦ $-x * z + \log(1 + e^x)$

⑧ $\max(x, 0) - x * z + \log(1 + e^{-\text{abs}(x)})$

$$\textcircled{4} \rightarrow \textcircled{5} \rightarrow C_1 z * A + (1-z)(x + A) \cdot C_2 \quad C_1 z A - C_2 z A + (1-z)x C_2$$

$$\frac{1}{1 + e^{-x}} = \frac{e^x}{e^x + 1} \quad \left| \quad \log\left(\frac{e^x + 1}{e^x}\right) = \log(e^x + 1) - \log(e^x)\right.$$

$$1 + e^{-x} = \frac{e^x + 1}{e^x}$$

$$= \log(e^x + 1) - x$$

Avec correction pour l'imbalance:

$$4 \quad B_p(z * \log(1 + e^{-x})) + B_N[(1-z) * (x + \log(1 + e^{-x}))] \quad x > 0$$

$$B_p(z * \log\left(\frac{e^x + 1}{e^x}\right)) + B_N[(1-z) * (x + \log\left(\frac{e^x + 1}{e^x}\right))] \quad x > 0$$

$$B_p(z * (\log(e^x + 1) - x)) + B_N[(1-z) * (\log(e^x + 1))] \quad x > 0$$

$$\left[B_p(z * (\log(1 + e^{-x}) + \min(0, x))) + B_N[(1-z) * (\max(0, x) + \log(e^{-x} + 1))] \right] \quad x > 0$$

tell - f sturn ... out

